tzprofiles intermediate proof

src/contracts_coq/tzprofiles.v
@@ -96,21 +96,13 @@ Module source.
   Definition contract_file := Eval cbv in (error.extract contract_file_M I).
 End source.
 
-(* Module annots. *)
-(*   Import String. *)
-(*   Definition rotateAuthentication : string := "%auth". *)
-(*   Definition rotateOwner : string := "%owner". *)
-(*   Definition rotateService : string := "%service". *)
-(* End annots. *)
-
 Definition parameter_ty := ep_leaf
   (pair (set (Cpair string (Cpair string bytes))) bool).
 
 Module tzprofiles(C:ContractContext).
 
-  (* (pair (pair (big_map %metadata string bytes) (address %owner)) *)
-  (*       (pair (pair %service (string %endpoint) (string %type_)) *)
-  (*             (address %verification_method))). *)
+(* storage (pair (pair (set %claims (pair (pair string bytes) string)) (string %contract_type)) *)
+(*         (pair (big_map %metadata string bytes) (address %owner))) ; *)
 Definition storage_ty :=
   (pair (pair (set (Cpair string (Cpair string bytes))) string)
         (pair (big_map string bytes) address)).
@@ -118,55 +110,393 @@ Definition storage_ty :=
 Definition tzprofiles : full_contract _ parameter_ty None storage_ty :=
   Eval cbv in contract_file_code source.contract_file.
 
+Import String.
+
+Definition raw_tzprofiles_iter_body :
+  instruction_seq
+    (Some
+       (ep_leaf
+          (pair
+             (set
+                (Cpair syntax_type.string (Cpair syntax_type.string bytes)))
+             (Comparable_type bool)), None)) false
+    (pair (Comparable_type syntax_type.string)
+       (pair (Comparable_type syntax_type.string) (Comparable_type bytes))
+     ::: set (Cpair syntax_type.string (Cpair syntax_type.string bytes))
+         ::: Comparable_type syntax_type.string
+             ::: pair (big_map syntax_type.string (Comparable_type bytes))
+                   (Comparable_type address)
+                 ::: Comparable_type bool ::: nil)
+    (set (Cpair syntax_type.string (Cpair syntax_type.string bytes))
+     ::: Comparable_type syntax_type.string
+         ::: pair (big_map syntax_type.string (Comparable_type bytes))
+               (Comparable_type address) ::: Comparable_type bool ::: nil).
+Proof.
+  pose (H := tzprofiles).
+  unfold tzprofiles in H.
+
+  do 25 match goal with
+  | _ := SEQ ?x ?y |- _ =>
+      (* pose x; *)
+      pose (H2 := y);
+      clear H;
+      rename H2 into H
+  end.
+
+  match goal with
+  | _ := SEQ ?x ?y |- _ =>
+      pose (H2 := x);
+      (* pose (H2 := y); *)
+      clear H;
+      rename H2 into H
+  end.
+
+  match goal with
+  | _ := ITER ?x |- _ =>
+      pose (H2 := x);
+      (* pose (H2 := y); *)
+      clear H;
+      rename H2 into H
+  end.
+
+  assumption.
+Defined.
+
+Definition tzprofiles_iter_body :
+  instruction_seq
+    (Some
+       (ep_leaf
+          (pair
+             (set
+                (Cpair syntax_type.string (Cpair syntax_type.string bytes)))
+             (Comparable_type bool)), None)) false
+    (pair (Comparable_type syntax_type.string)
+       (pair (Comparable_type syntax_type.string) (Comparable_type bytes))
+     ::: set (Cpair syntax_type.string (Cpair syntax_type.string bytes))
+         ::: Comparable_type syntax_type.string
+             ::: pair (big_map syntax_type.string (Comparable_type bytes))
+                   (Comparable_type address)
+                 ::: Comparable_type bool ::: nil)
+    (set (Cpair syntax_type.string (Cpair syntax_type.string bytes))
+     ::: Comparable_type syntax_type.string
+         ::: pair (big_map syntax_type.string (Comparable_type bytes))
+               (Comparable_type address) ::: Comparable_type bool ::: nil) :=
+  Eval lazy in raw_tzprofiles_iter_body.
+
+Definition raw_tzprofiles_iter :
+ instruction
+   (Some
+      (ep_leaf
+         (pair
+            (set
+               (Cpair syntax_type.string (Cpair syntax_type.string bytes)))
+            (Comparable_type bool)), None)) false
+   (set (Cpair syntax_type.string (Cpair syntax_type.string bytes))
+    ::: set (Cpair syntax_type.string (Cpair syntax_type.string bytes))
+        ::: Comparable_type syntax_type.string
+            ::: pair (big_map syntax_type.string (Comparable_type bytes))
+                  (Comparable_type address)
+                ::: Comparable_type bool ::: nil)
+   (set (Cpair syntax_type.string (Cpair syntax_type.string bytes))
+    ::: Comparable_type syntax_type.string
+        ::: pair (big_map syntax_type.string (Comparable_type bytes))
+              (Comparable_type address) ::: Comparable_type bool ::: nil).
+Proof.
+  pose (H := tzprofiles).
+  unfold tzprofiles in H.
+
+  do 25 match goal with
+  | _ := SEQ ?x ?y |- _ =>
+      (* pose x; *)
+      pose (H2 := y);
+      clear H;
+      rename H2 into H
+  end.
+
+  match goal with
+  | _ := SEQ ?x ?y |- _ =>
+      pose (H2 := x);
+      (* pose (H2 := y); *)
+      clear H;
+      rename H2 into H
+  end.
+
+  assumption.
+Defined.
+
+Definition tzprofiles_iter :
+ instruction
+   (Some
+      (ep_leaf
+         (pair
+            (set
+               (Cpair syntax_type.string (Cpair syntax_type.string bytes)))
+            (Comparable_type bool)), None)) false
+   (set (Cpair syntax_type.string (Cpair syntax_type.string bytes))
+    ::: set (Cpair syntax_type.string (Cpair syntax_type.string bytes))
+        ::: Comparable_type syntax_type.string
+            ::: pair (big_map syntax_type.string (Comparable_type bytes))
+                  (Comparable_type address)
+                ::: Comparable_type bool ::: nil)
+   (set (Cpair syntax_type.string (Cpair syntax_type.string bytes))
+    ::: Comparable_type syntax_type.string
+        ::: pair (big_map syntax_type.string (Comparable_type bytes))
+              (Comparable_type address) ::: Comparable_type bool ::: nil) :=
+  Eval lazy in raw_tzprofiles_iter.
+
+Lemma tzprofiles_iter_to_body_correct :
+  tzprofiles_iter = @ITER _ _ _
+    (Mk_iter _ _
+      (Iter_variant_set (Cpair _ (Cpair _ (Comparable_type_simple _)))))
+    _
+    tzprofiles_iter_body.
+Proof. reflexivity. Qed.
+
+
+
 Module semantics := Semantics C. Import semantics.
 Export semantics.
 
+(* Check eval_seq. *)
+
+Lemma tzprofiles_iter_body_raw_spec_correct
+      (env : @proto_env (Some (parameter_ty, None)))
+      (* (x0 : data (pair *)
+      (*   (Comparable_type syntax_type.string) *)
+      (*   (pair (Comparable_type syntax_type.string) (Comparable_type bytes)))) *)
+
+      (x0_1 : data (Comparable_type syntax_type.string))
+      (x0_2 : data (Comparable_type syntax_type.string))
+      (x0_3 : data (Comparable_type bytes))
+
+      (x1 : data (set (Cpair syntax_type.string (Cpair syntax_type.string bytes))))
+      (x2 : data (Comparable_type syntax_type.string))
+      (x3 : data (pair
+        (big_map syntax_type.string (Comparable_type bytes))
+        (Comparable_type address)))
+      (x4 : data (Comparable_type bool))
+
+      (y0 : data (set (Cpair syntax_type.string (Cpair syntax_type.string bytes))))
+      (y1 : data (Comparable_type syntax_type.string))
+      (y2 : data (pair (big_map syntax_type.string (Comparable_type bytes))
+                 (Comparable_type address)))
+      (y3 : data (Comparable_type bool))
+      (fuel : Datatypes.nat) :
+  eval_seq env tzprofiles_iter_body (6 + fuel)
+    ((x0_1, (x0_2, x0_3)), (x1, (x2, (x3, (x4, tt))))) =
+    Return (y0, (y1, (y2, (y3, tt))))
+  <->
+  (update _ _ _ (Update_variant_set (Cpair syntax_type.string (Cpair syntax_type.string bytes)))
+    (x0_1, (x0_2, x0_3)) x4 x1,
+  (x2, (x3, (x4, tt)))) =
+  (y0,
+  (y1, (y2, (y3, tt)))).
+Proof.
+  remember (6 + fuel) as fuel2.
+  assert (6 <= fuel2) by lia.
+  rewrite return_precond.
+  rewrite eval_seq_precond_correct.
+  unfold eval_seq_precond.
+  unfold tzprofiles_iter_body.
+
+  do 6 (more_fuel; simpl).
+  reflexivity.
+Qed.
+
+(* Lemma tzprofiles_iter_raw_spec_correct *)
+(*       (env : @proto_env (Some (parameter_ty, None))) *)
+
+(*       (x0 : data (set (Cpair syntax_type.string (Cpair syntax_type.string bytes)))) *)
+(*       (x1 : data (set (Cpair syntax_type.string (Cpair syntax_type.string bytes)))) *)
+(*       (x2 : data (Comparable_type syntax_type.string)) *)
+(*       (x3 : data (pair (big_map syntax_type.string (Comparable_type bytes)) (Comparable_type address))) *)
+(*       (x4 : data (Comparable_type bool)) *)
+
+(*       (y0 : data (set (Cpair syntax_type.string (Cpair syntax_type.string bytes)))) *)
+(*       (y1 : data (Comparable_type syntax_type.string)) *)
+(*       (y2 : data (pair (big_map syntax_type.string (Comparable_type bytes)) *)
+(*                  (Comparable_type address))) *)
+(*       (y3 : data (Comparable_type bool)) *)
+(*       (fuel : Datatypes.nat) : *)
+
+(*   eval env tzprofiles_iter (6 + fuel) *)
+(*     (x0, (x1, (x2, (x3, (x4, tt))))) = *)
+(*     Return (y0, (y1, (y2, (y3, tt)))) *)
+(*   <-> *)
+(*   false. *)
+(* Proof. *)
+(*   remember (6 + fuel) as fuel2. *)
+(*   assert (6 <= fuel2) by lia. *)
+(*   rewrite return_precond. *)
+(*   (1* rewrite eval_seq_precond_correct. *1) *)
+(*   (1* unfold eval_seq_precond. *1) *)
+(*   unfold tzprofiles_iter. *)
+
+
+(*   Check (precond_iter_bounded *)
+(*     (@Some (entrypoint_tree * Datatypes.option annotation) (parameter_ty, @None annotation)) *)
+(*     false *)
+(*     env *)
+(*   ). *)
+
+(*   Check set.destruct. *)
+(*   Locate set.set. *)
+(*   Print set.set. *)
+(*   Print data_aux. *)
+(*   Print data. *)
+(*   Locate "{ _ | _ }". *)
+(*   Check proj1_sig. *)
+(*   Locate proj1. *)
+(*   (1* Search (sig -> _). *1) *)
+(*   Check (forall a (xs : set.set (comparable_data a) (compare a)), proj1_sig xs = nil). *)
+(*   (1* List.list. *1) *)
+(*   (1* Search set.set List.list. *1) *)
+
+(*   Check TODO_prove_precond_ITER_ignores_set_and_treats_it_like_the_list_in_sig. *)
+
+(*   precond (eval env (ITER body) fuel (xs, input_stack)) psi = *)
+(*   precond (eval env (ITER body) fuel (proj1_sig xs, input_stack)) psi. *)
+
+
+(*   Lemma precond_iter_bounded st tff env a (l : data (list a)) A (body : instruction_seq st tff (a ::: A) A) *)
+(*         fuel_bound body_spec *)
+(*     (Hbody_correct : *)
+(*        forall fuel (x : data a) (input_stack : stack A) (psi : stack A -> Prop), *)
+(*         fuel_bound <= fuel -> *)
+(*         precond (eval_seq env body fuel (x, input_stack)) psi *)
+(*         <-> body_spec psi x input_stack) *)
+(*     (Hbody_spec_extensional : *)
+(*        forall psi1 psi2 x input_stack, *)
+(*         (forall x, psi1 x <-> psi2 x) -> *)
+(*         body_spec psi1 x input_stack <-> body_spec psi2 x input_stack) : *)
+
+
+
+(*   Can't use precond_iter_bounded since it's specialized to lists. *)
+(*   It should be possible to replace lists with sets in it somehow. *)
+
+(*   Search ITER. *)
+(*   _ *)
+
+
+(*   rewrite precond_iter_bounded. *)
+(*   precond_iter_bounded *)
+
+
+
+(*   do 6 (more_fuel; simpl). *)
+(*   reflexivity. *)
+(* Qed. *)
+
+(* Definition tzprofiles_iter : *)
+(*  instruction *)
+(*    (Some *)
+(*       (ep_leaf *)
+(*          (pair *)
+(*             (set *)
+(*                (Cpair syntax_type.string (Cpair syntax_type.string bytes))) *)
+(*             (Comparable_type bool)), None)) false *)
+(*    (set (Cpair syntax_type.string (Cpair syntax_type.string bytes)) *)
+(*     ::: set (Cpair syntax_type.string (Cpair syntax_type.string bytes)) *)
+(*         ::: Comparable_type syntax_type.string *)
+(*             ::: pair (big_map syntax_type.string (Comparable_type bytes)) *)
+(*                   (Comparable_type address) *)
+(*                 ::: Comparable_type bool ::: nil) *)
+(*    (set (Cpair syntax_type.string (Cpair syntax_type.string bytes)) *)
+(*     ::: Comparable_type syntax_type.string *)
+(*         ::: pair (big_map syntax_type.string (Comparable_type bytes)) *)
+(*               (Comparable_type address) ::: Comparable_type bool ::: nil) := *)
+(*   Eval lazy in raw_tzprofiles_iter. *)
+
+
+(* Check TODO_apply_tzprofiles_iter_body_to_iter_spec. *)
+
+
+(* Print tzprofiles_iter_body. *)
+
+(* Lemma ok : Datatypes.unit. *)
+(* Proof. *)
+(*   pose (H := tzprofiles). *)
+(*   unfold tzprofiles in H. *)
+
+(*   Check @SEQ. *)
+(*   (1* Set Printing All. *1) *)
+(*   do 25 match goal with *)
+(*   | _ := SEQ ?x ?y |- _ => *)
+(*       (1* pose x; *1) *)
+(*       pose (H2 := y); *)
+(*       clear H; *)
+(*       rename H2 into H *)
+(*   end. *)
+
+(*   match goal with *)
+(*   | _ := SEQ ?x ?y |- _ => *)
+(*       pose (H2 := x); *)
+(*       (1* pose (H2 := y); *1) *)
+(*       clear H; *)
+(*       rename H2 into H *)
+(*   end. *)
+
+(*   match goal with *)
+(*   | _ := ITER ?x |- _ => *)
+(*       pose (H2 := x); *)
+(*       (1* pose (H2 := y); *1) *)
+(*       clear H; *)
+(*       rename H2 into H *)
+(*   end. *)
+
+
+(*   Check SEQ. *)
+(*   Search SEQ. *)
+(*   Print tzprofiles. *)
+
+
 (* Definition tzprofiles_spec_helper *)
 (*            (env : @proto_env (Some (parameter_ty, None))) *)
+(*            (claims : data (set (Cpair string (Cpair string bytes)))) *)
+(*            (contract_type : data string) *)
 (*            (metadata : data (big_map string bytes)) *)
 (*            (owner : data address) *)
-(*            (endpoint : data string) *)
-(*            (type_ : data string) *)
-(*            (verification_method : data address) *)
 (*            (param : data parameter_ty) *)
 (*            (new_storage : data storage_ty) *)
 (*            (returned_operations : data (list operation)) := *)
 (*   let storage : data storage_ty := *)
-(*     ((metadata, owner), *)
-(*           ((endpoint, type_), verification_method)) in *)
+(*     ((claims, contract_type), *)
+(*       (metadata, owner)) in *)
 
 (*   negb (comparison_to_int (address_compare (sender env) owner) =? 0)%Z = false /\ *)
 (*   (comparison_to_int (tez.compare (amount env) (0 ~Mutez)) >? 0)%Z = false /\ *)
-(*   match param with *)
-(*   | inl rotateOwner => *)
-(*       (nil, (metadata, rotateOwner, (endpoint, type_, verification_method)), tt) = *)
-(*       (returned_operations, new_storage, tt) *)
-(*   | inr (inl rotateAuth) => *)
-(*       (nil, (metadata, owner, (endpoint, type_, rotateAuth)), tt) = *)
-(*       (returned_operations, new_storage, tt) *)
-(*   | inr (inr rotateService) => *)
-(*       (nil, (metadata, owner, (rotateService, verification_method)), tt) = *)
-(*       (returned_operations, new_storage, tt) *)
-(*   end. *)
+(*   false. *)
+
+(*   (1* match param with *1) *)
+(*   (1* | inl rotateOwner => *1) *)
+(*   (1*     (nil, (metadata, rotateOwner, (endpoint, type_, verification_method)), tt) = *1) *)
+(*   (1*     (returned_operations, new_storage, tt) *1) *)
+(*   (1* | inr (inl rotateAuth) => *1) *)
+(*   (1*     (nil, (metadata, owner, (endpoint, type_, rotateAuth)), tt) = *1) *)
+(*   (1*     (returned_operations, new_storage, tt) *1) *)
+(*   (1* | inr (inr rotateService) => *1) *)
+(*   (1*     (nil, (metadata, owner, (rotateService, verification_method)), tt) = *1) *)
+(*   (1*     (returned_operations, new_storage, tt) *1) *)
+(*   (1* end. *1) *)
 
 (* Lemma tzprofiles_spec_helper_correct *)
 (*       (env : @proto_env (Some (parameter_ty, None))) *)
+(*       (claims : data (set (Cpair string (Cpair string bytes)))) *)
+(*       (contract_type : data string) *)
 (*       (metadata : data (big_map string bytes)) *)
 (*       (owner : data address) *)
-(*       (endpoint : data string) *)
-(*       (type_ : data string) *)
-(*       (verification_method : data address) *)
 (*       (param : data parameter_ty) *)
 (*       (new_storage : data storage_ty) *)
 (*       (returned_operations : data (list operation)) *)
 (*       (fuel : Datatypes.nat) : *)
 (*   let storage : data storage_ty := *)
-(*     ((metadata, owner), *)
-(*           ((endpoint, type_), verification_method)) in *)
+(*     ((claims, contract_type), *)
+(*       (metadata, owner)) in *)
 (*   eval_seq env tzprofiles (100 + fuel) ((param, storage), tt) = *)
 (*     Return ((returned_operations, new_storage), tt) *)
-(*   <-> tzprofiles_spec_helper env metadata owner endpoint type_ verification_method *)
-(*     param new_storage returned_operations. *)
+(*   <-> tzprofiles_spec_helper env claims contract_type metadata owner param *)
+(*     new_storage returned_operations. *)
 (* Proof. *)
 (*   intro Hfuel. *)
 (*   remember (100 + fuel) as fuel2. *)
@@ -175,129 +505,204 @@ Export semantics.
 (*   rewrite eval_seq_precond_correct. *)
 (*   unfold eval_seq_precond. *)
 (*   unfold tzprofiles_spec_helper. *)
+
+(*   (more_fuel; simpl). *)
+(*   (more_fuel; simpl). *)
+(*   (more_fuel; simpl). *)
+
+(*   apply and_iff_compat_l. *)
+
+(*   destruct param as (claim_set & add_remove). *)
+
+(*   (more_fuel; simpl). *)
+(*   rewrite precond_iter_fun. *)
+(*   precond_iter_bounded. *)
+
+(*   Search UPDATE. *)
+(*   Check update. *)
+(*   Print update_variant. *)
+
+(*   Check (fun a => update _ _ _ (Update_variant_set a)). *)
+
+(*   Check (fun a b => *)
+(*     List.fold_left *)
+(*       (fun (memo : data (set a)) x => update _ _ _ (Update_variant_set a) x b memo)). *)
+
+(* fun a : comparable_type => update a bool (set a) (Update_variant_set a) *)
+(*      : forall a : comparable_type, *)
+(*        comparable_data a -> data bool -> data (set a) -> data (set a) *)
+
+
+(*   Fixpoint fold_left (l:list B) (a0:A) : A := *)
+(*     match l with *)
+(*       | nil => a0 *)
+(*       | cons b t => fold_left t (f a0 b) *)
+(*     end. *)
+
+
+(*   Check TODO_define_update. *)
+
+(*   Definition update a b c (v : update_variant a b c) : *)
+(*     comparable_data a -> data b -> data c -> data c := *)
+(*     match v with *)
+(*     | Update_variant_set a => *)
+(*       set.update _ _ (compare_eq_iff a) (lt_trans a) (gt_trans a) *)
+(*     | Update_variant_map k v => *)
+(*       map.update _ _ _ (compare_eq_iff k) (lt_trans k) (gt_trans k) *)
+(*     | Update_variant_bigmap k _ => *)
+(*       map.update _ _ _ (compare_eq_iff k) (lt_trans k) (gt_trans k) *)
+(*     end. *)
+
+
+(*   Search update. *)
+(*   _ *)
+(*   (1* (more_fuel; simpl). *1) *)
+(*   (1* (more_fuel; simpl). *1) *)
+(*   (1* (more_fuel; simpl). *1) *)
+(*   (1* (more_fuel; simpl). *1) *)
+(*   (1* (more_fuel; simpl). *1) *)
+(*   (1* (more_fuel; simpl). *1) *)
+
+
+(*   _ *)
+(*   (1* (more_fuel; simpl). *1) *)
+(*   (1* (more_fuel; simpl). *1) *)
+
+(*   Search (_ /\ _ <-> _ /\ _). *)
+
+(*   _ *)
+(*   (1* (more_fuel; simpl). *1) *)
+(*   (1* (more_fuel; simpl). *1) *)
+(*   (1* (more_fuel; simpl). *1) *)
+(*   (1* (more_fuel; simpl). *1) *)
+(*   (1* (more_fuel; simpl). *1) *)
+(*   (1* (more_fuel; simpl). *1) *)
+
+
+(*   (do 3 (more_fuel; simpl); reflexivity). *)
 (*   destruct param as [[rotateAuth | rotateOwner] | rotateService]; *)
 (*   (do 3 (more_fuel; simpl); reflexivity). *)
 (* Qed. *)
 
-(* Definition tzprofiles_spec *)
-(*            (env : @proto_env (Some (parameter_ty, None))) *)
-(*            (metadata : data (big_map string bytes)) *)
-(*            (owner : data address) *)
-(*            (endpoint : data string) *)
-(*            (type_ : data string) *)
-(*            (verification_method : data address) *)
-(*            (param : data parameter_ty) *)
-(*            (new_storage : data storage_ty) *)
-(*            (returned_operations : data (list operation)) := *)
-(*   let storage : data storage_ty := *)
-(*     ((metadata, owner), *)
-(*     ((endpoint, type_), *)
-(*       verification_method)) in *)
+(* (1* Definition tzprofiles_spec *1) *)
+(* (1*            (env : @proto_env (Some (parameter_ty, None))) *1) *)
+(* (1*            (metadata : data (big_map string bytes)) *1) *)
+(* (1*            (owner : data address) *1) *)
+(* (1*            (endpoint : data string) *1) *)
+(* (1*            (type_ : data string) *1) *)
+(* (1*            (verification_method : data address) *1) *)
+(* (1*            (param : data parameter_ty) *1) *)
+(* (1*            (new_storage : data storage_ty) *1) *)
+(* (1*            (returned_operations : data (list operation)) := *1) *)
+(* (1*   let storage : data storage_ty := *1) *)
+(* (1*     ((metadata, owner), *1) *)
+(* (1*     ((endpoint, type_), *1) *)
+(* (1*       verification_method)) in *1) *)
 
-(*   match new_storage with *)
-(*   | ((new_metadata, new_owner), *)
-(*     ((new_endpoint, new_type_), *)
-(*       new_verification_method)) => *)
+(* (1*   match new_storage with *1) *)
+(* (1*   | ((new_metadata, new_owner), *1) *)
+(* (1*     ((new_endpoint, new_type_), *1) *)
+(* (1*       new_verification_method)) => *1) *)
 
-(*     sender env = owner /\ *)
+(* (1*     sender env = owner /\ *1) *)
 
-(*     (int64bv.to_Z (tez.to_int64 (amount env)) <= 0)%Z /\ *)
+(* (1*     (int64bv.to_Z (tez.to_int64 (amount env)) <= 0)%Z /\ *1) *)
 
-(*     returned_operations = nil /\ *)
-(*     new_metadata = metadata /\ *)
+(* (1*     returned_operations = nil /\ *1) *)
+(* (1*     new_metadata = metadata /\ *1) *)
 
-(*     match param with *)
-(*     | inl rotateOwner => *)
-(*         new_owner = rotateOwner /\ *)
-(*         new_endpoint = endpoint /\ *)
-(*         new_type_ = type_ /\ *)
-(*         new_verification_method = verification_method *)
-(*     | inr (inl rotateAuth) => *)
-(*         new_owner = owner /\ *)
-(*         new_endpoint = endpoint /\ *)
-(*         new_type_ = type_ /\ *)
-(*         new_verification_method = rotateAuth *)
-(*     | inr (inr (rotateEndpoint, rotateType)) => *)
-(*         new_owner = owner /\ *)
-(*         new_endpoint = rotateEndpoint /\ *)
-(*         new_type_ = rotateType /\ *)
-(*         new_verification_method = verification_method *)
-(*     end *)
-(*   end. *)
+(* (1*     match param with *1) *)
+(* (1*     | inl rotateOwner => *1) *)
+(* (1*         new_owner = rotateOwner /\ *1) *)
+(* (1*         new_endpoint = endpoint /\ *1) *)
+(* (1*         new_type_ = type_ /\ *1) *)
+(* (1*         new_verification_method = verification_method *1) *)
+(* (1*     | inr (inl rotateAuth) => *1) *)
+(* (1*         new_owner = owner /\ *1) *)
+(* (1*         new_endpoint = endpoint /\ *1) *)
+(* (1*         new_type_ = type_ /\ *1) *)
+(* (1*         new_verification_method = rotateAuth *1) *)
+(* (1*     | inr (inr (rotateEndpoint, rotateType)) => *1) *)
+(* (1*         new_owner = owner /\ *1) *)
+(* (1*         new_endpoint = rotateEndpoint /\ *1) *)
+(* (1*         new_type_ = rotateType /\ *1) *)
+(* (1*         new_verification_method = verification_method *1) *)
+(* (1*     end *1) *)
+(* (1*   end. *1) *)
 
-(* Lemma tzprofiles_spec_correct *)
-(*       (env : @proto_env (Some (parameter_ty, None))) *)
-(*       (metadata : data (big_map string bytes)) *)
-(*       (owner : data address) *)
-(*       (endpoint : data string) *)
-(*       (type_ : data string) *)
-(*       (verification_method : data address) *)
-(*       (param : data parameter_ty) *)
-(*       (new_storage : data storage_ty) *)
-(*       (returned_operations : data (list operation)) *)
-(*       (fuel : Datatypes.nat) : *)
-(*   let storage : data storage_ty := *)
-(*     ((metadata, owner), *)
-(*           ((endpoint, type_), verification_method)) in *)
-(*   eval_seq env tzprofiles (100 + fuel) ((param, storage), tt) = *)
-(*     Return ((returned_operations, new_storage), tt) *)
-(*   <-> tzprofiles_spec env metadata owner endpoint type_ verification_method *)
-(*     param new_storage returned_operations. *)
-(* Proof. *)
-(*   Arguments Nat.add : simpl never. *)
-(*   simpl. *)
-(*   Arguments Nat.add : simpl nomatch. *)
+(* (1* Lemma tzprofiles_spec_correct *1) *)
+(* (1*       (env : @proto_env (Some (parameter_ty, None))) *1) *)
+(* (1*       (metadata : data (big_map string bytes)) *1) *)
+(* (1*       (owner : data address) *1) *)
+(* (1*       (endpoint : data string) *1) *)
+(* (1*       (type_ : data string) *1) *)
+(* (1*       (verification_method : data address) *1) *)
+(* (1*       (param : data parameter_ty) *1) *)
+(* (1*       (new_storage : data storage_ty) *1) *)
+(* (1*       (returned_operations : data (list operation)) *1) *)
+(* (1*       (fuel : Datatypes.nat) : *1) *)
+(* (1*   let storage : data storage_ty := *1) *)
+(* (1*     ((metadata, owner), *1) *)
+(* (1*           ((endpoint, type_), verification_method)) in *1) *)
+(* (1*   eval_seq env tzprofiles (100 + fuel) ((param, storage), tt) = *1) *)
+(* (1*     Return ((returned_operations, new_storage), tt) *1) *)
+(* (1*   <-> tzprofiles_spec env metadata owner endpoint type_ verification_method *1) *)
+(* (1*     param new_storage returned_operations. *1) *)
+(* (1* Proof. *1) *)
+(* (1*   Arguments Nat.add : simpl never. *1) *)
+(* (1*   simpl. *1) *)
+(* (1*   Arguments Nat.add : simpl nomatch. *1) *)
 
-(*   rewrite tzprofiles_spec_helper_correct. *)
-(*   unfold tzprofiles_spec_helper. *)
-(*   unfold tzprofiles_spec. *)
+(* (1*   rewrite tzprofiles_spec_helper_correct. *1) *)
+(* (1*   unfold tzprofiles_spec_helper. *1) *)
+(* (1*   unfold tzprofiles_spec. *1) *)
 
-(*   rewrite address_compare_iff, tez_not_gt_0. *)
+(* (1*   rewrite address_compare_iff, tez_not_gt_0. *1) *)
 
-(*   destruct param as [rotateOwner | [rotateAuth | (rotateEndpoint & rotateType)]]. *)
+(* (1*   destruct param as [rotateOwner | [rotateAuth | (rotateEndpoint & rotateType)]]. *1) *)
 
-(*   - split; intro H. *)
-(*     + repeat match goal with *)
-(*       | H : _ /\ _ |- _ => destruct H *)
-(*       | H : _ = _ |- _ => inversion H; destruct H *)
-(*       | |- (let (x, y) := ?z in _) => destruct z *)
-(*       end; *)
-(*       tauto. *)
-(*     + repeat match goal with *)
-(*       | H : (let (x, y) := ?z in _) |- _ => destruct z *)
-(*       | H : _ /\ _ |- _ => destruct H *)
-(*       end; *)
-(*       repeat split; try congruence; *)
-(*       repeat f_equal; intuition. *)
+(* (1*   - split; intro H. *1) *)
+(* (1*     + repeat match goal with *1) *)
+(* (1*       | H : _ /\ _ |- _ => destruct H *1) *)
+(* (1*       | H : _ = _ |- _ => inversion H; destruct H *1) *)
+(* (1*       | |- (let (x, y) := ?z in _) => destruct z *1) *)
+(* (1*       end; *1) *)
+(* (1*       tauto. *1) *)
+(* (1*     + repeat match goal with *1) *)
+(* (1*       | H : (let (x, y) := ?z in _) |- _ => destruct z *1) *)
+(* (1*       | H : _ /\ _ |- _ => destruct H *1) *)
+(* (1*       end; *1) *)
+(* (1*       repeat split; try congruence; *1) *)
+(* (1*       repeat f_equal; intuition. *1) *)
 
-(*   - split; intro H. *)
-(*     + repeat match goal with *)
-(*       | H : _ /\ _ |- _ => destruct H *)
-(*       | H : _ = _ |- _ => inversion H; destruct H *)
-(*       | |- (let (x, y) := ?z in _) => destruct z *)
-(*       end; *)
-(*       tauto. *)
-(*     + repeat match goal with *)
-(*       | H : (let (x, y) := ?z in _) |- _ => destruct z *)
-(*       | H : _ /\ _ |- _ => destruct H *)
-(*       end; *)
-(*       repeat split; try congruence; *)
-(*       repeat f_equal; intuition. *)
+(* (1*   - split; intro H. *1) *)
+(* (1*     + repeat match goal with *1) *)
+(* (1*       | H : _ /\ _ |- _ => destruct H *1) *)
+(* (1*       | H : _ = _ |- _ => inversion H; destruct H *1) *)
+(* (1*       | |- (let (x, y) := ?z in _) => destruct z *1) *)
+(* (1*       end; *1) *)
+(* (1*       tauto. *1) *)
+(* (1*     + repeat match goal with *1) *)
+(* (1*       | H : (let (x, y) := ?z in _) |- _ => destruct z *1) *)
+(* (1*       | H : _ /\ _ |- _ => destruct H *1) *)
+(* (1*       end; *1) *)
+(* (1*       repeat split; try congruence; *1) *)
+(* (1*       repeat f_equal; intuition. *1) *)
 
-(*   - split; intro H. *)
-(*     + repeat match goal with *)
-(*       | H : _ /\ _ |- _ => destruct H *)
-(*       | H : _ = _ |- _ => inversion H; destruct H *)
-(*       | |- (let (x, y) := ?z in _) => destruct z *)
-(*       end; *)
-(*       tauto. *)
-(*     + repeat match goal with *)
-(*       | H : (let (x, y) := ?z in _) |- _ => destruct z *)
-(*       | H : _ /\ _ |- _ => destruct H *)
-(*       end. *)
-(*       repeat split; try congruence; *)
-(*       repeat f_equal; intuition. *)
-(* Qed. *)
+(* (1*   - split; intro H. *1) *)
+(* (1*     + repeat match goal with *1) *)
+(* (1*       | H : _ /\ _ |- _ => destruct H *1) *)
+(* (1*       | H : _ = _ |- _ => inversion H; destruct H *1) *)
+(* (1*       | |- (let (x, y) := ?z in _) => destruct z *1) *)
+(* (1*       end; *1) *)
+(* (1*       tauto. *1) *)
+(* (1*     + repeat match goal with *1) *)
+(* (1*       | H : (let (x, y) := ?z in _) |- _ => destruct z *1) *)
+(* (1*       | H : _ /\ _ |- _ => destruct H *1) *)
+(* (1*       end. *1) *)
+(* (1*       repeat split; try congruence; *1) *)
+(* (1*       repeat f_equal; intuition. *1) *)
+(* (1* Qed. *1) *)
 
 End tzprofiles.
 
