src/contracts_coq/vesting_tez.v
@@ -19,441 +19,441 @@
 (* FROM, OUT OF OR IN CONNECTION WITH THE SOFTWARE OR THE USE OR OTHER *)
 (* DEALINGS IN THE SOFTWARE. *)
 
-Require Import Coq.Classes.EquivDec.
-Require Import Michocoq.macros.
-Require Import syntax macros main semantics comparable util.
-Require Import ZArith.
-Require Import Lia.
-Import error entrypoints.
-Require List.
-Require tez.
-Require map.
-Require String.
+(* Require Import Coq.Classes.EquivDec. *)
+(* Require Import Michocoq.macros. *)
+(* Require Import syntax macros main semantics comparable util. *)
+(* Require Import ZArith. *)
+(* Require Import Lia. *)
+(* Import error entrypoints. *)
+(* Require List. *)
+(* Require tez. *)
+(* Require map. *)
+(* Require String. *)
 
-Require vesting_tez_string.
+(* Require vesting_tez_string. *)
 
-Module source.
-  Definition contract_file_M :=
-    main.contract_file_M vesting_tez_string.vesting_tez_s 10.
+(* Module source. *)
+(*   Definition contract_file_M := *)
+(*     main.contract_file_M vesting_tez_string.vesting_tez_s 10. *)
 
-  Definition contract_file := Eval cbv in (error.extract contract_file_M I).
-End source.
+(*   Definition contract_file := Eval cbv in (error.extract contract_file_M I). *)
+(* End source. *)
 
-Module annots.
-  Import String.
-  Definition setDelegate : string := "%setDelegate".
-  Definition vest : string := "%vest".
-End annots.
+(* Module annots. *)
+(*   Import String. *)
+(*   Definition setDelegate : string := "%setDelegate". *)
+(*   Definition vest : string := "%vest". *)
+(* End annots. *)
 
-Definition parameter_ty :=
-  (ep_node (ep_leaf (option key_hash)) (Some annots.setDelegate)
-      (ep_leaf nat) (Some annots.vest)
-).
+(* Definition parameter_ty := *)
+(*   (ep_node (ep_leaf (option key_hash)) (Some annots.setDelegate) *)
+(*       (ep_leaf nat) (Some annots.vest) *)
+(* ). *)
 
-Module vesting_tez(C:ContractContext).
+(* Module vesting_tez(C:ContractContext). *)
 
-Definition storage_ty :=
-  (pair (pair address address)
-        (pair nat
-              (pair timestamp (pair nat nat)))).
+(* Definition storage_ty := *)
+(*   (pair (pair address address) *)
+(*         (pair nat *)
+(*               (pair timestamp (pair nat nat)))). *)
 
-Definition vesting_tez : full_contract _ parameter_ty None storage_ty :=
-  Eval cbv in contract_file_code source.contract_file.
+(* Definition vesting_tez : full_contract _ parameter_ty None storage_ty := *)
+(*   Eval cbv in contract_file_code source.contract_file. *)
 
-Module semantics := Semantics C. Import semantics.
+(* Module semantics := Semantics C. Import semantics. *)
 
-Definition vesting_tez_spec
-           (env : @proto_env (Some (parameter_ty, None)))
-           (target : data address)
-           (delegateAdmin : data address)
-           (vested : data nat)
-           (epoch : data timestamp)
-           (secondsPerTick : data nat)
-           (tokensPerTick : data nat)
-           (param : data parameter_ty)
-           (new_storage : data storage_ty)
-           (returned_operations : data (list operation)) :=
-  let storage : data storage_ty :=
-    ((target, delegateAdmin),
-    (vested, (epoch, (secondsPerTick, tokensPerTick)))) in
+(* Definition vesting_tez_spec *)
+(*            (env : @proto_env (Some (parameter_ty, None))) *)
+(*            (target : data address) *)
+(*            (delegateAdmin : data address) *)
+(*            (vested : data nat) *)
+(*            (epoch : data timestamp) *)
+(*            (secondsPerTick : data nat) *)
+(*            (tokensPerTick : data nat) *)
+(*            (param : data parameter_ty) *)
+(*            (new_storage : data storage_ty) *)
+(*            (returned_operations : data (list operation)) := *)
+(*   let storage : data storage_ty := *)
+(*     ((target, delegateAdmin), *)
+(*     (vested, (epoch, (secondsPerTick, tokensPerTick)))) in *)
 
-  (* %setDelegate: the admin may set the delegate *)
-  match param with
-  | inl kh =>
-    sender env = delegateAdmin /\
-    new_storage = storage /\
-    returned_operations = (set_delegate kh :: nil)%list
+(*   (1* %setDelegate: the admin may set the delegate *1) *)
+(*   match param with *)
+(*   | inl kh => *)
+(*     sender env = delegateAdmin /\ *)
+(*     new_storage = storage /\ *)
+(*     returned_operations = (set_delegate kh :: nil)%list *)
 
-  (* %vest: anybody can flush tokens *)
-  (* this does not modify the storage and produces a 'transfer_tokens'. *)
-  | inr to_flush =>
-    secondsPerTick <> 0%N /\
-    (Z.of_N (to_flush + vested) <= (now env - epoch) / Z.of_N secondsPerTick)%Z /\
-    new_storage =
-      ((target, delegateAdmin),
-      ((to_flush + vested)%N, (epoch, (secondsPerTick, tokensPerTick)))) /\
-    exists target_contract, contract_ None unit I target = Some target_contract /\
-    let tokens_to_flush := (to_flush * tokensPerTick)%N in
-    exists pf,
-    let tez_to_flush :=
-      tez.of_Z_safe
-        (Z.of_N tokens_to_flush)
-        pf in
-    returned_operations =
-      (transfer_tokens unit I tt tez_to_flush target_contract :: nil)%list
-  end.
+(*   (1* %vest: anybody can flush tokens *1) *)
+(*   (1* this does not modify the storage and produces a 'transfer_tokens'. *1) *)
+(*   | inr to_flush => *)
+(*     secondsPerTick <> 0%N /\ *)
+(*     (Z.of_N (to_flush + vested) <= (now env - epoch) / Z.of_N secondsPerTick)%Z /\ *)
+(*     new_storage = *)
+(*       ((target, delegateAdmin), *)
+(*       ((to_flush + vested)%N, (epoch, (secondsPerTick, tokensPerTick)))) /\ *)
+(*     exists target_contract, contract_ None unit I target = Some target_contract /\ *)
+(*     let tokens_to_flush := (to_flush * tokensPerTick)%N in *)
+(*     exists pf, *)
+(*     let tez_to_flush := *)
+(*       tez.of_Z_safe *)
+(*         (Z.of_N tokens_to_flush) *)
+(*         pf in *)
+(*     returned_operations = *)
+(*       (transfer_tokens unit I tt tez_to_flush target_contract :: nil)%list *)
+(*   end. *)
 
-Definition vesting_tez_spec_helper
-           (env : @proto_env (Some (parameter_ty, None)))
-           (target : data address)
-           (delegateAdmin : data address)
-           (vested : data nat)
-           (epoch : data timestamp)
-           (secondsPerTick : data nat)
-           (tokensPerTick : data nat)
-           (param : data parameter_ty)
-           (new_storage : data storage_ty)
-           (returned_operations : data (list operation)) :=
-  let storage : data storage_ty :=
-    ((target, delegateAdmin),
-    (vested, (epoch, (secondsPerTick, tokensPerTick)))) in
+(* Definition vesting_tez_spec_helper *)
+(*            (env : @proto_env (Some (parameter_ty, None))) *)
+(*            (target : data address) *)
+(*            (delegateAdmin : data address) *)
+(*            (vested : data nat) *)
+(*            (epoch : data timestamp) *)
+(*            (secondsPerTick : data nat) *)
+(*            (tokensPerTick : data nat) *)
+(*            (param : data parameter_ty) *)
+(*            (new_storage : data storage_ty) *)
+(*            (returned_operations : data (list operation)) := *)
+(*   let storage : data storage_ty := *)
+(*     ((target, delegateAdmin), *)
+(*     (vested, (epoch, (secondsPerTick, tokensPerTick)))) in *)
 
-  (* %setDelegate: the admin may set the delegate *)
-  match param with
-  | inl kh =>
-    sender env = delegateAdmin /\
-    new_storage = storage /\
-    returned_operations = (set_delegate kh :: nil)%list
+(*   (1* %setDelegate: the admin may set the delegate *1) *)
+(*   match param with *)
+(*   | inl kh => *)
+(*     sender env = delegateAdmin /\ *)
+(*     new_storage = storage /\ *)
+(*     returned_operations = (set_delegate kh :: nil)%list *)
 
-  (* %vest: anybody can flush tokens *)
-  (* this does not modify the storage and produces a 'transfer_tokens'. *)
-  | inr to_flush =>
-    let expected_new_storage : data storage_ty :=
-      ((target, delegateAdmin),
-      ((to_flush + vested)%N, (epoch, (secondsPerTick, tokensPerTick)))) in
-    exists target_contract, contract_ None unit I target = Some target_contract /\
-    secondsPerTick <> N0 /\
-    is_true (comparison_to_int (
-        to_flush ?= Z.to_N ((now env - epoch) / Z.of_N secondsPerTick - Z.of_N vested)
-      )%N <=? 0)%Z /\
-    is_true ((now env - epoch) / Z.of_N secondsPerTick - Z.of_N vested >=? 0)%Z /\
-    let m_tez_to_flush := tez.of_Z (Z.of_N (to_flush * tokensPerTick)) in
-    exists m_tez_to_flush_ok : is_true (success m_tez_to_flush),
-    let tez_to_flush := extract m_tez_to_flush m_tez_to_flush_ok in
-    new_storage = expected_new_storage /\
-    returned_operations =
-      (transfer_tokens unit I tt tez_to_flush target_contract :: nil)%list
-  end.
+(*   (1* %vest: anybody can flush tokens *1) *)
+(*   (1* this does not modify the storage and produces a 'transfer_tokens'. *1) *)
+(*   | inr to_flush => *)
+(*     let expected_new_storage : data storage_ty := *)
+(*       ((target, delegateAdmin), *)
+(*       ((to_flush + vested)%N, (epoch, (secondsPerTick, tokensPerTick)))) in *)
+(*     exists target_contract, contract_ None unit I target = Some target_contract /\ *)
+(*     secondsPerTick <> N0 /\ *)
+(*     is_true (comparison_to_int ( *)
+(*         to_flush ?= Z.to_N ((now env - epoch) / Z.of_N secondsPerTick - Z.of_N vested) *)
+(*       )%N <=? 0)%Z /\ *)
+(*     is_true ((now env - epoch) / Z.of_N secondsPerTick - Z.of_N vested >=? 0)%Z /\ *)
+(*     let m_tez_to_flush := tez.of_Z (Z.of_N (to_flush * tokensPerTick)) in *)
+(*     exists m_tez_to_flush_ok : is_true (success m_tez_to_flush), *)
+(*     let tez_to_flush := extract m_tez_to_flush m_tez_to_flush_ok in *)
+(*     new_storage = expected_new_storage /\ *)
+(*     returned_operations = *)
+(*       (transfer_tokens unit I tt tez_to_flush target_contract :: nil)%list *)
+(*   end. *)
 
-Lemma shim_simplify_flush_vested_ineqs (vested : data nat)
-                                       (to_flush : data nat)
-                                       (z : Z) :
-  (to_flush <= Z.to_N (z - Z.of_N vested))%N /\ (0 <= z - Z.of_N vested)%Z <->
-  (Z.of_N (to_flush + vested) <= z)%Z.
-Proof.
-  split; intro H.
-  - destruct H as (Hsum & Hpos).
-    refine (proj2 (Z2N.inj_le _ _ _ _) _).
-    + rewrite <- (N2Z.id to_flush) in Hsum.
-      apply (proj2 (Z2N.inj_le _ _ (N2Z.is_nonneg _) Hpos)) in Hsum.
-      refine (Z.le_trans _ _ _ (N2Z.is_nonneg _) _).
-      refine (proj2 (Z2N.inj_le _ _ (N2Z.is_nonneg _) (N2Z.is_nonneg _)) _).
-      do 2 rewrite N2Z.id.
-      exact (N.le_add_r _ _).
-    + apply Zle_0_minus_le in Hpos.
-      exact (Z.le_trans _ _ _ (N2Z.is_nonneg _) Hpos).
-    + rewrite N2Z.id.
-      rewrite Z2N.inj_sub in Hsum by exact (N2Z.is_nonneg _).
-      rewrite N2Z.id in Hsum.
-      apply (N.add_le_mono_r _ _ vested) in Hsum.
-      rewrite N.sub_add in Hsum.
-      * assumption.
-      * apply Zle_0_minus_le in Hpos.
-        apply (proj1 (Z2N.inj_le _ _
-         (N2Z.is_nonneg _)
-         (Z.le_trans _ _ _ (N2Z.is_nonneg _) Hpos)
-        )) in Hpos.
-        rewrite N2Z.id in Hpos.
-        rewrite N.sub_add in Hsum; assumption.
-  - pose (z_nonneg := Z.le_trans _ _ _ (N2Z.is_nonneg _) H).
-    split.
-    + pose (H' := H).
-      apply (proj1 (Z2N.inj_le _ _ (N2Z.is_nonneg _) z_nonneg)) in H'.
-      rewrite N2Z.id in H'.
-      rewrite (Z2N.inj_sub _ _ (N2Z.is_nonneg _)).
-      rewrite N2Z.id.
-      exact (N.le_add_le_sub_r _ _ _ H').
-    + refine (Zle_minus_le_0 _ _ _).
-      pose (H' := H).
-      rewrite N2Z.inj_add in H'.
-      rewrite <- (Z.add_0_r z) in H'.
-      rewrite <- Z.add_comm in H'.
-      refine (Z.le_le_add_le _ _ _ _ (N2Z.is_nonneg _) H').
-Qed.
+(* Lemma shim_simplify_flush_vested_ineqs (vested : data nat) *)
+(*                                        (to_flush : data nat) *)
+(*                                        (z : Z) : *)
+(*   (to_flush <= Z.to_N (z - Z.of_N vested))%N /\ (0 <= z - Z.of_N vested)%Z <-> *)
+(*   (Z.of_N (to_flush + vested) <= z)%Z. *)
+(* Proof. *)
+(*   split; intro H. *)
+(*   - destruct H as (Hsum & Hpos). *)
+(*     refine (proj2 (Z2N.inj_le _ _ _ _) _). *)
+(*     + rewrite <- (N2Z.id to_flush) in Hsum. *)
+(*       apply (proj2 (Z2N.inj_le _ _ (N2Z.is_nonneg _) Hpos)) in Hsum. *)
+(*       refine (Z.le_trans _ _ _ (N2Z.is_nonneg _) _). *)
+(*       refine (proj2 (Z2N.inj_le _ _ (N2Z.is_nonneg _) (N2Z.is_nonneg _)) _). *)
+(*       do 2 rewrite N2Z.id. *)
+(*       exact (N.le_add_r _ _). *)
+(*     + apply Zle_0_minus_le in Hpos. *)
+(*       exact (Z.le_trans _ _ _ (N2Z.is_nonneg _) Hpos). *)
+(*     + rewrite N2Z.id. *)
+(*       rewrite Z2N.inj_sub in Hsum by exact (N2Z.is_nonneg _). *)
+(*       rewrite N2Z.id in Hsum. *)
+(*       apply (N.add_le_mono_r _ _ vested) in Hsum. *)
+(*       rewrite N.sub_add in Hsum. *)
+(*       * assumption. *)
+(*       * apply Zle_0_minus_le in Hpos. *)
+(*         apply (proj1 (Z2N.inj_le _ _ *)
+(*          (N2Z.is_nonneg _) *)
+(*          (Z.le_trans _ _ _ (N2Z.is_nonneg _) Hpos) *)
+(*         )) in Hpos. *)
+(*         rewrite N2Z.id in Hpos. *)
+(*         rewrite N.sub_add in Hsum; assumption. *)
+(*   - pose (z_nonneg := Z.le_trans _ _ _ (N2Z.is_nonneg _) H). *)
+(*     split. *)
+(*     + pose (H' := H). *)
+(*       apply (proj1 (Z2N.inj_le _ _ (N2Z.is_nonneg _) z_nonneg)) in H'. *)
+(*       rewrite N2Z.id in H'. *)
+(*       rewrite (Z2N.inj_sub _ _ (N2Z.is_nonneg _)). *)
+(*       rewrite N2Z.id. *)
+(*       exact (N.le_add_le_sub_r _ _ _ H'). *)
+(*     + refine (Zle_minus_le_0 _ _ _). *)
+(*       pose (H' := H). *)
+(*       rewrite N2Z.inj_add in H'. *)
+(*       rewrite <- (Z.add_0_r z) in H'. *)
+(*       rewrite <- Z.add_comm in H'. *)
+(*       refine (Z.le_le_add_le _ _ _ _ (N2Z.is_nonneg _) H'). *)
+(* Qed. *)
 
-(* In coq 8.11+, the proof of the 'assert' below is just 'lia'. *)
-Lemma vesting_tez_spec_helper_flush_helper
-      (now_env : data timestamp)
-      (vested : data nat)
-      (epoch : data timestamp)
-      (secondsPerTick : data nat)
-      (to_flush : data nat) :
-  is_true (comparison_to_int (
-      to_flush ?= Z.to_N ((now_env - epoch) / Z.of_N secondsPerTick - Z.of_N vested)
-    )%N <=? 0)%Z /\
-  is_true ((now_env - epoch) / Z.of_N secondsPerTick - Z.of_N vested >=? 0)%Z <->
-  (Z.of_N (to_flush + vested) <= (now_env - epoch) / Z.of_N secondsPerTick)%Z.
-Proof.
-  rewrite N_comparison_to_int_leb.
-  refine (iff_trans (and_both_0 _ _) _).
-  - refine (iff_trans (IT_eq_iff _) _);
-    exact (N.leb_le _ _).
-  - refine (iff_trans (IT_eq_iff _) _);
-    exact (Z.geb_le _ _).
-  - apply shim_simplify_flush_vested_ineqs.
-Qed.
+(* (1* In coq 8.11+, the proof of the 'assert' below is just 'lia'. *1) *)
+(* Lemma vesting_tez_spec_helper_flush_helper *)
+(*       (now_env : data timestamp) *)
+(*       (vested : data nat) *)
+(*       (epoch : data timestamp) *)
+(*       (secondsPerTick : data nat) *)
+(*       (to_flush : data nat) : *)
+(*   is_true (comparison_to_int ( *)
+(*       to_flush ?= Z.to_N ((now_env - epoch) / Z.of_N secondsPerTick - Z.of_N vested) *)
+(*     )%N <=? 0)%Z /\ *)
+(*   is_true ((now_env - epoch) / Z.of_N secondsPerTick - Z.of_N vested >=? 0)%Z <-> *)
+(*   (Z.of_N (to_flush + vested) <= (now_env - epoch) / Z.of_N secondsPerTick)%Z. *)
+(* Proof. *)
+(*   rewrite N_comparison_to_int_leb. *)
+(*   refine (iff_trans (and_both_0 _ _) _). *)
+(*   - refine (iff_trans (IT_eq_iff _) _); *)
+(*     exact (N.leb_le _ _). *)
+(*   - refine (iff_trans (IT_eq_iff _) _); *)
+(*     exact (Z.geb_le _ _). *)
+(*   - apply shim_simplify_flush_vested_ineqs. *)
+(* Qed. *)
 
-Lemma of_Z_success z : success (tez.of_Z z) <-> Bool.Is_true (tez.in_bound z).
-Proof.
-  unfold tez.of_Z.
-  destruct (tez.in_bound z); simpl; intuition.
-Qed.
+(* Lemma of_Z_success z : success (tez.of_Z z) <-> Bool.Is_true (tez.in_bound z). *)
+(* Proof. *)
+(*   unfold tez.of_Z. *)
+(*   destruct (tez.in_bound z); simpl; intuition. *)
+(* Qed. *)
 
-Lemma return_extract {A} (m : M A) H : Return (extract m H) = m.
-Proof.
-  destruct m.
-  - contradiction.
-  - destruct H.
-    reflexivity.
-Qed.
+(* Lemma return_extract {A} (m : M A) H : Return (extract m H) = m. *)
+(* Proof. *)
+(*   destruct m. *)
+(*   - contradiction. *)
+(*   - destruct H. *)
+(*     reflexivity. *)
+(* Qed. *)
 
-Lemma return_extract_2 {A} (m : M A) a H : m = Return a -> extract m H = a.
-Proof.
-  intro; subst; simpl.
-  destruct H.
-  reflexivity.
-Qed.
+(* Lemma return_extract_2 {A} (m : M A) a H : m = Return a -> extract m H = a. *)
+(* Proof. *)
+(*   intro; subst; simpl. *)
+(*   destruct H. *)
+(*   reflexivity. *)
+(* Qed. *)
 
-Lemma vesting_tez_spec_helper_correct
-      (env : @proto_env (Some (parameter_ty, None)))
-      (target : data address)
-      (delegateAdmin : data address)
-      (vested : data nat)
-      (epoch : data timestamp)
-      (secondsPerTick : data nat)
-      (tokensPerTick : data nat)
-      (param : data parameter_ty)
-      (new_storage : data storage_ty)
-      (returned_operations : data (list operation)) :
-  vesting_tez_spec_helper
-    env
-    target
-    delegateAdmin
-    vested
-    epoch
-    secondsPerTick
-    tokensPerTick
-    param
-    new_storage
-    returned_operations
-  <-> vesting_tez_spec
-    env
-    target
-    delegateAdmin
-    vested
-    epoch
-    secondsPerTick
-    tokensPerTick
-    param
-    new_storage
-    returned_operations.
-Proof.
-  unfold vesting_tez_spec_helper.
-  unfold vesting_tez_spec.
-  destruct param; (tauto || idtac).
-  do 2 refine (iff_trans _ (and_assoc _ _ _)).
-  refine (iff_trans _ (iff_sym ex_and_comm)).
-  refine (forall_ex _).
-  intros [target_address target_o target_type_eq].
-  refine (iff_trans _ (and_comm _ _)).
-  refine (iff_trans _ (iff_sym (and_assoc _ _ _))).
-  refine (and_both _).
-  refine (iff_trans _ (and_comm _ _)).
-  do 2 refine (iff_trans _ (iff_sym (and_assoc _ _ _))).
-  refine (and_both _).
-  refine (iff_trans (iff_sym (and_assoc _ _ _)) _).
-  refine (and_both_0 (vesting_tez_spec_helper_flush_helper _ _ _ _ _) _).
-  refine (iff_trans (iff_sym ex_and_comm) _).
-  refine (and_both _).
-  split; intros (pf & Hpf).
-  - exists (proj1 (of_Z_success _) pf).
-    rewrite Hpf.
-    do 3 f_equal.
-    apply unreturn.
-    rewrite <- tez.of_Z_is_safe.
-    apply return_extract.
-  - exists (proj2 (of_Z_success _) pf).
-    rewrite Hpf.
-    do 3 f_equal.
-    apply unreturn.
-    rewrite <- tez.of_Z_is_safe.
-    symmetry.
-    apply return_extract.
-Qed.
+(* Lemma vesting_tez_spec_helper_correct *)
+(*       (env : @proto_env (Some (parameter_ty, None))) *)
+(*       (target : data address) *)
+(*       (delegateAdmin : data address) *)
+(*       (vested : data nat) *)
+(*       (epoch : data timestamp) *)
+(*       (secondsPerTick : data nat) *)
+(*       (tokensPerTick : data nat) *)
+(*       (param : data parameter_ty) *)
+(*       (new_storage : data storage_ty) *)
+(*       (returned_operations : data (list operation)) : *)
+(*   vesting_tez_spec_helper *)
+(*     env *)
+(*     target *)
+(*     delegateAdmin *)
+(*     vested *)
+(*     epoch *)
+(*     secondsPerTick *)
+(*     tokensPerTick *)
+(*     param *)
+(*     new_storage *)
+(*     returned_operations *)
+(*   <-> vesting_tez_spec *)
+(*     env *)
+(*     target *)
+(*     delegateAdmin *)
+(*     vested *)
+(*     epoch *)
+(*     secondsPerTick *)
+(*     tokensPerTick *)
+(*     param *)
+(*     new_storage *)
+(*     returned_operations. *)
+(* Proof. *)
+(*   unfold vesting_tez_spec_helper. *)
+(*   unfold vesting_tez_spec. *)
+(*   destruct param; (tauto || idtac). *)
+(*   do 2 refine (iff_trans _ (and_assoc _ _ _)). *)
+(*   refine (iff_trans _ (iff_sym ex_and_comm)). *)
+(*   refine (forall_ex _). *)
+(*   intros [target_address target_o target_type_eq]. *)
+(*   refine (iff_trans _ (and_comm _ _)). *)
+(*   refine (iff_trans _ (iff_sym (and_assoc _ _ _))). *)
+(*   refine (and_both _). *)
+(*   refine (iff_trans _ (and_comm _ _)). *)
+(*   do 2 refine (iff_trans _ (iff_sym (and_assoc _ _ _))). *)
+(*   refine (and_both _). *)
+(*   refine (iff_trans (iff_sym (and_assoc _ _ _)) _). *)
+(*   refine (and_both_0 (vesting_tez_spec_helper_flush_helper _ _ _ _ _) _). *)
+(*   refine (iff_trans (iff_sym ex_and_comm) _). *)
+(*   refine (and_both _). *)
+(*   split; intros (pf & Hpf). *)
+(*   - exists (proj1 (of_Z_success _) pf). *)
+(*     rewrite Hpf. *)
+(*     do 3 f_equal. *)
+(*     apply unreturn. *)
+(*     rewrite <- tez.of_Z_is_safe. *)
+(*     apply return_extract. *)
+(*   - exists (proj2 (of_Z_success _) pf). *)
+(*     rewrite Hpf. *)
+(*     do 3 f_equal. *)
+(*     apply unreturn. *)
+(*     rewrite <- tez.of_Z_is_safe. *)
+(*     symmetry. *)
+(*     apply return_extract. *)
+(* Qed. *)
 
-Lemma vesting_tez_helper_correct
-      (env : @proto_env (Some (parameter_ty, None)))
-      (target : data address)
-      (delegateAdmin : data address)
-      (vested : data nat)
-      (epoch : data timestamp)
-      (secondsPerTick : data nat)
-      (tokensPerTick : data nat)
-      (param : data parameter_ty)
-      (new_storage : data storage_ty)
-      (returned_operations : data (list operation))
-      (fuel : Datatypes.nat) :
-  let storage : data storage_ty :=
-    ((target, delegateAdmin),
-    (vested, (epoch, (secondsPerTick, tokensPerTick)))) in
-  eval_seq env vesting_tez (100 + fuel) ((param, storage), tt) = Return ((returned_operations, new_storage), tt)
-  <-> vesting_tez_spec_helper
-    env
-    target
-    delegateAdmin
-    vested
-    epoch
-    secondsPerTick
-    tokensPerTick
-    param
-    new_storage
-    returned_operations.
-Proof.
-  intro storage.
-  remember (100 + fuel) as fuel2.
-  assert (100 <= fuel2) by lia.
-  rewrite return_precond.
-  rewrite eval_seq_precond_correct.
-  unfold eval_seq_precond.
-  unfold vesting_tez_spec_helper.
-  destruct param as [kh | to_flush].
-  {
-    do 17 (more_fuel; simpl).
-    rewrite Z.eqb_eq.
-    rewrite comparison_to_int_Eq.
-    rewrite (compare_eq_iff address).
-    apply and_both.
-    unfold storage.
-    rewrite and_pair_eq.
-    rewrite and_comm.
-    apply and_left; [reflexivity|].
-    unfold data; simpl.
-    rewrite and_pair_eq.
-    intuition.
-  }
-  {
-    do 5 (more_fuel; simpl).
-    split.
-    - intros ((q, r), (H1, H2)).
-      destruct (q - Z.of_N vested >=? 0)%Z eqn:Hdiff.
-      + destruct H2 as (y, (Hy, (Hflush, (c, (Hc, Hm))))).
-        assert (y = Z.to_N (q - Z.of_N vested)) by congruence.
-        subst y.
-        clear Hy.
-        rewrite precond_exists in Hm.
-        destruct Hm as (z, (Hz, H2)).
-        rewrite and_pair_eq in H2.
-        unfold data in H2; simpl in H2.
-        rewrite and_pair_eq in H2.
-        destruct H2 as ((H2, H3), _).
-        subst.
-        change (tez.of_Z (1%Z * Z.of_N (to_flush * tokensPerTick)) = Return z) in Hz.
-        rewrite Z.mul_1_l in Hz.
-        rewrite Hz.
-        simpl.
-        exists c.
-        split; [assumption|].
-        split; [apply ediv_Z_correct in H1; lia|].
-        assert (q = ((now env - epoch) / Z.of_N secondsPerTick)%Z).
-        * rewrite ediv_Z_correct in H1.
-          destruct H1 as (H1, H2).
-          apply (Zdiv_unique _ _ _ (Z.of_N r)); [nia|symmetry; assumption].
-        * split; [|split].
-          -- subst.
-             apply Bool.Is_true_eq_left.
-             apply Hflush.
-          -- apply Bool.Is_true_eq_left.
-             congruence.
-          -- exists I; split; reflexivity.
-      + destruct H2 as (y, (Habsurd, _)).
-        discriminate.
-    - intros (target_contract, (Ht, (Hspt, (Hflush, (Hdiff, (Hsuccess, He)))))).
-      exists (((now env - epoch) / Z.of_N secondsPerTick), Z.to_N ((now env - epoch) mod Z.of_N secondsPerTick))%Z.
-      split.
-      + assert (Z.of_N secondsPerTick > 0)%Z as Hpos by lia.
-        assert (0 <= ((now env - epoch) mod Z.of_N secondsPerTick))%Z as Hneg
-            by (apply Z_mod_lt; assumption).
-        assert (Z.of_N (Z.to_N ((now env - epoch) mod Z.of_N secondsPerTick)) = ((now env - epoch) mod Z.of_N secondsPerTick))%Z
-          as Hid by (apply Z2N.id; assumption).
-        rewrite ediv_Z_correct.
-        split.
-        * symmetry.
-          etransitivity; [apply (Z_div_mod_eq _ _ Hpos)|].
-          rewrite Hid.
-          reflexivity.
-        * rewrite Hid.
-          replace (Z.abs (Z.of_N secondsPerTick)) with (Z.of_N secondsPerTick).
-          -- apply Z_mod_lt. assumption.
-          -- lia.
-      + apply Bool.Is_true_eq_true in Hdiff.
-        rewrite Hdiff.
-        eexists.
-        split; [reflexivity|].
-        apply Bool.Is_true_eq_true in Hflush.
-        split; [assumption|].
-        eexists.
-        split; [eassumption|].
-        destruct (success_eq_return_rev _ _ Hsuccess) as (m, Hm).
-        change (tez.to_Z _) with 1%Z.
-        rewrite Z.mul_1_l.
-        rewrite Hm.
-        apply (return_extract_2 _ _ Hsuccess) in Hm.
-        simpl.
-        destruct He; subst.
-        reflexivity.
-  }
-Qed.
+(* Lemma vesting_tez_helper_correct *)
+(*       (env : @proto_env (Some (parameter_ty, None))) *)
+(*       (target : data address) *)
+(*       (delegateAdmin : data address) *)
+(*       (vested : data nat) *)
+(*       (epoch : data timestamp) *)
+(*       (secondsPerTick : data nat) *)
+(*       (tokensPerTick : data nat) *)
+(*       (param : data parameter_ty) *)
+(*       (new_storage : data storage_ty) *)
+(*       (returned_operations : data (list operation)) *)
+(*       (fuel : Datatypes.nat) : *)
+(*   let storage : data storage_ty := *)
+(*     ((target, delegateAdmin), *)
+(*     (vested, (epoch, (secondsPerTick, tokensPerTick)))) in *)
+(*   eval_seq env vesting_tez (100 + fuel) ((param, storage), tt) = Return ((returned_operations, new_storage), tt) *)
+(*   <-> vesting_tez_spec_helper *)
+(*     env *)
+(*     target *)
+(*     delegateAdmin *)
+(*     vested *)
+(*     epoch *)
+(*     secondsPerTick *)
+(*     tokensPerTick *)
+(*     param *)
+(*     new_storage *)
+(*     returned_operations. *)
+(* Proof. *)
+(*   intro storage. *)
+(*   remember (100 + fuel) as fuel2. *)
+(*   assert (100 <= fuel2) by lia. *)
+(*   rewrite return_precond. *)
+(*   rewrite eval_seq_precond_correct. *)
+(*   unfold eval_seq_precond. *)
+(*   unfold vesting_tez_spec_helper. *)
+(*   destruct param as [kh | to_flush]. *)
+(*   { *)
+(*     do 17 (more_fuel; simpl). *)
+(*     rewrite Z.eqb_eq. *)
+(*     rewrite comparison_to_int_Eq. *)
+(*     rewrite (compare_eq_iff address). *)
+(*     apply and_both. *)
+(*     unfold storage. *)
+(*     rewrite and_pair_eq. *)
+(*     rewrite and_comm. *)
+(*     apply and_left; [reflexivity|]. *)
+(*     unfold data; simpl. *)
+(*     rewrite and_pair_eq. *)
+(*     intuition. *)
+(*   } *)
+(*   { *)
+(*     do 5 (more_fuel; simpl). *)
+(*     split. *)
+(*     - intros ((q, r), (H1, H2)). *)
+(*       destruct (q - Z.of_N vested >=? 0)%Z eqn:Hdiff. *)
+(*       + destruct H2 as (y, (Hy, (Hflush, (c, (Hc, Hm))))). *)
+(*         assert (y = Z.to_N (q - Z.of_N vested)) by congruence. *)
+(*         subst y. *)
+(*         clear Hy. *)
+(*         rewrite precond_exists in Hm. *)
+(*         destruct Hm as (z, (Hz, H2)). *)
+(*         rewrite and_pair_eq in H2. *)
+(*         unfold data in H2; simpl in H2. *)
+(*         rewrite and_pair_eq in H2. *)
+(*         destruct H2 as ((H2, H3), _). *)
+(*         subst. *)
+(*         change (tez.of_Z (1%Z * Z.of_N (to_flush * tokensPerTick)) = Return z) in Hz. *)
+(*         rewrite Z.mul_1_l in Hz. *)
+(*         rewrite Hz. *)
+(*         simpl. *)
+(*         exists c. *)
+(*         split; [assumption|]. *)
+(*         split; [apply ediv_Z_correct in H1; lia|]. *)
+(*         assert (q = ((now env - epoch) / Z.of_N secondsPerTick)%Z). *)
+(*         * rewrite ediv_Z_correct in H1. *)
+(*           destruct H1 as (H1, H2). *)
+(*           apply (Zdiv_unique _ _ _ (Z.of_N r)); [nia|symmetry; assumption]. *)
+(*         * split; [|split]. *)
+(*           -- subst. *)
+(*              apply Bool.Is_true_eq_left. *)
+(*              apply Hflush. *)
+(*           -- apply Bool.Is_true_eq_left. *)
+(*              congruence. *)
+(*           -- exists I; split; reflexivity. *)
+(*       + destruct H2 as (y, (Habsurd, _)). *)
+(*         discriminate. *)
+(*     - intros (target_contract, (Ht, (Hspt, (Hflush, (Hdiff, (Hsuccess, He)))))). *)
+(*       exists (((now env - epoch) / Z.of_N secondsPerTick), Z.to_N ((now env - epoch) mod Z.of_N secondsPerTick))%Z. *)
+(*       split. *)
+(*       + assert (Z.of_N secondsPerTick > 0)%Z as Hpos by lia. *)
+(*         assert (0 <= ((now env - epoch) mod Z.of_N secondsPerTick))%Z as Hneg *)
+(*             by (apply Z_mod_lt; assumption). *)
+(*         assert (Z.of_N (Z.to_N ((now env - epoch) mod Z.of_N secondsPerTick)) = ((now env - epoch) mod Z.of_N secondsPerTick))%Z *)
+(*           as Hid by (apply Z2N.id; assumption). *)
+(*         rewrite ediv_Z_correct. *)
+(*         split. *)
+(*         * symmetry. *)
+(*           etransitivity; [apply (Z_div_mod_eq _ _ Hpos)|]. *)
+(*           rewrite Hid. *)
+(*           reflexivity. *)
+(*         * rewrite Hid. *)
+(*           replace (Z.abs (Z.of_N secondsPerTick)) with (Z.of_N secondsPerTick). *)
+(*           -- apply Z_mod_lt. assumption. *)
+(*           -- lia. *)
+(*       + apply Bool.Is_true_eq_true in Hdiff. *)
+(*         rewrite Hdiff. *)
+(*         eexists. *)
+(*         split; [reflexivity|]. *)
+(*         apply Bool.Is_true_eq_true in Hflush. *)
+(*         split; [assumption|]. *)
+(*         eexists. *)
+(*         split; [eassumption|]. *)
+(*         destruct (success_eq_return_rev _ _ Hsuccess) as (m, Hm). *)
+(*         change (tez.to_Z _) with 1%Z. *)
+(*         rewrite Z.mul_1_l. *)
+(*         rewrite Hm. *)
+(*         apply (return_extract_2 _ _ Hsuccess) in Hm. *)
+(*         simpl. *)
+(*         destruct He; subst. *)
+(*         reflexivity. *)
+(*   } *)
+(* Qed. *)
 
-Lemma vesting_tez_correct
-      (env : @proto_env (Some (parameter_ty, None)))
-      (target : data address)
-      (delegateAdmin : data address)
-      (vested : data nat)
-      (epoch : data timestamp)
-      (secondsPerTick : data nat)
-      (tokensPerTick : data nat)
-      (param : data parameter_ty)
-      (new_storage : data storage_ty)
-      (returned_operations : data (list operation))
-      (fuel : Datatypes.nat) :
-  let storage : data storage_ty :=
-    ((target, delegateAdmin),
-    (vested, (epoch, (secondsPerTick, tokensPerTick)))) in
-  eval_seq env vesting_tez (100 + fuel) ((param, storage), tt) = Return ((returned_operations, new_storage), tt)
-  <-> vesting_tez_spec
-    env
-    target
-    delegateAdmin
-    vested
-    epoch
-    secondsPerTick
-    tokensPerTick
-    param
-    new_storage
-    returned_operations.
-Proof.
-refine (iff_trans (vesting_tez_helper_correct _ _ _ _ _ _ _ _ _ _ _) _).
-exact (vesting_tez_spec_helper_correct _ _ _ _ _ _ _ _ _ _).
-Qed.
+(* Lemma vesting_tez_correct *)
+(*       (env : @proto_env (Some (parameter_ty, None))) *)
+(*       (target : data address) *)
+(*       (delegateAdmin : data address) *)
+(*       (vested : data nat) *)
+(*       (epoch : data timestamp) *)
+(*       (secondsPerTick : data nat) *)
+(*       (tokensPerTick : data nat) *)
+(*       (param : data parameter_ty) *)
+(*       (new_storage : data storage_ty) *)
+(*       (returned_operations : data (list operation)) *)
+(*       (fuel : Datatypes.nat) : *)
+(*   let storage : data storage_ty := *)
+(*     ((target, delegateAdmin), *)
+(*     (vested, (epoch, (secondsPerTick, tokensPerTick)))) in *)
+(*   eval_seq env vesting_tez (100 + fuel) ((param, storage), tt) = Return ((returned_operations, new_storage), tt) *)
+(*   <-> vesting_tez_spec *)
+(*     env *)
+(*     target *)
+(*     delegateAdmin *)
+(*     vested *)
+(*     epoch *)
+(*     secondsPerTick *)
+(*     tokensPerTick *)
+(*     param *)
+(*     new_storage *)
+(*     returned_operations. *)
+(* Proof. *)
+(* refine (iff_trans (vesting_tez_helper_correct _ _ _ _ _ _ _ _ _ _ _) _). *)
+(* exact (vesting_tez_spec_helper_correct _ _ _ _ _ _ _ _ _ _). *)
+(* Qed. *)
 
-End vesting_tez.
+(* End vesting_tez. *)
